src/Memory.v
@@ -1,0 +1,35 @@
+From Coq Require Import
+     Arith.PeanoNat
+     Logic.FunctionalExtensionality.
+
+Require Export Heapster.Permissions.
+
+(* Memory model *)
+Definition addr : Set := nat * nat.
+Lemma addr_dec : forall (a b : addr), {a = b} + {a <> b}.
+Proof.
+  intros [a1 a2] [b1 b2].
+  destruct (Nat.eq_dec a1 b1); destruct (Nat.eq_dec a2 b2); subst; auto.
+  - right. intros H. inversion H; subst. apply n. reflexivity.
+  - right. intros H. inversion H; subst. apply n. reflexivity.
+  - right. intros H. inversion H; subst. apply n. reflexivity.
+Qed.
+
+Lemma addr_neq_cases (b b' o o' : nat) :
+  (b, o) <> (b', o') -> b <> b' \/ o <> o'.
+Proof.
+  intros.
+  destruct (Nat.eq_dec b b'); destruct (Nat.eq_dec o o'); subst; auto.
+Qed.
+
+Inductive SByte :=
+| Byte : nat -> SByte
+| Ptr : addr -> SByte
+(* | SUndef : SByte. *)
+.
+Definition mem_block := nat -> option SByte.
+
+Variant logical_block :=
+| LBlock (size : nat) (bytes : mem_block) : logical_block.
+
+Definition memory := nat -> option logical_block.
